```math
\left( \begin{matrix}
a_{11} & \dots & a_{1m} \\
\vdots & \ddots & \vdots \\
a_{11} & \dots & a_{1m} \\
\end{matrix} \right)
\cdot 
\left( \begin{matrix}
x_1\\ \vdots \\
x_i = 0 \\ \vdots\\
x_j = 1\\ \vdots\\
x_m\\
\end{matrix} \right)
=
\left( \begin{matrix}
\sum_{k=1}^m {a_{1k} \cdot x_k}\\ \vdots\\
\sum_{k=1}^m {a_{nk} \cdot x_k}\\
\end{matrix} \right)
``` 
---
```math
\left( \begin{matrix}
a_{11} & \dots & a_{1m} \\
\vdots & \ddots & \vdots \\
a_{11} & \dots & a_{1m} \\
\end{matrix} \right)
\cdot 
\left( \begin{matrix}
y_1 = x_1\\ \vdots \\
y_i = 1 \\ \vdots\\
y_j = 0\\ \vdots\\
y_m = x_m\\
\end{matrix} \right)
=
\left( \begin{matrix}
\sum_{k=1}^m {a_{1k} \cdot x_k} + a_{1i} - a_{1j}\\ \vdots\\
\sum_{k=1}^m {a_{nk} \cdot x_k} + a_{ni} - a_{nj}\\
\end{matrix} \right)
